fstar/MLS.Crypto.Derived.fsti
@@ -13,3 +13,4 @@ val ciphersuite_to_nt: ciphersuite -> result cipher_suite_nt
 
 val expand_with_label: ciphersuite -> secret:bytes -> label:bytes -> context:bytes -> len:size_nat -> result (lbytes len)
 val derive_secret: cs:ciphersuite -> secret:bytes -> label:bytes -> result (lbytes (kdf_length cs))
+val make_hash_ref: ciphersuite -> bytes -> result (lbytes 16)
