fstar/MLS.Result.fst
@@ -1,8 +1,6 @@
 module MLS.Result
-open Lib.Sequence
 
-
-#set-options "--z3rlimit_factor 2"
+#set-options "--fuel 0 --ifuel 0"
 
 type result 'a =
   | Success: v:'a -> result 'a
@@ -13,29 +11,35 @@ let return (a:'a) : result 'a = Success a
 let internal_failure (#a:Type) (s:string): result a = InternalError s
 let error (#a:Type) (s:string): result a = ProtocolError s
 
+#push-options "--ifuel 1"
 //TODO unfold? (to remove all the lambdas in the spec and in the generated code)
 let bind (a:result 'a) (f:'a -> result 'b) : result 'b =
   match a with
   | Success x -> f x
   | InternalError x -> InternalError x
   | ProtocolError x -> ProtocolError x
+#pop-options
 
 let from_option (s:string) (x:option 'a): result 'a =
   match x with
   | None -> ProtocolError s
   | Some x -> Success x
 
-let rec mapM (f:('a -> result 'b)) (l:list 'a): result (list 'b) =
+#push-options "--ifuel 1 --fuel 1"
+let rec mapM (f:('a -> result 'b)) (l:list 'a): result (res:list 'b{List.Tot.length res == List.Tot.length l}) =
   match l with
   | [] -> return []
   | h::t ->
     fh <-- f h;
     ft <-- mapM f t;
-    return (fh::ft)
+    return #(res:list 'b{List.Tot.length res == List.Tot.length l}) (fh::ft)
+#pop-options
 
+#push-options "--ifuel 1 --fuel 1"
 let rec fold_leftM (f:'a -> 'b -> result 'a) (x:'a) (l:list 'b): Tot (result 'a) (decreases l) =
   match l with
   | [] -> return x
   | h::t ->
     new_x <-- f x h;
     fold_leftM f new_x t
+#pop-options
