fstar/MLS.TreeSync.KeyPackageRef.fst
@@ -1,0 +1,30 @@
+module MLS.TreeSync.KeyPackageRef
+
+open MLS.Utils
+open MLS.Tree
+open MLS.TreeSync.Types
+open MLS.NetworkTypes
+open MLS.NetworkBinder
+open MLS.Crypto
+open MLS.Parser
+open MLS.Result
+
+val leaf_package_to_kp_ref: cs:ciphersuite -> leaf_package_t -> result (key_package_ref_nt)
+let leaf_package_to_kp_ref cs lp =
+  kp <-- treesync_to_keypackage cs lp;
+  let kp_bytes = ps_key_package.serialize kp in
+  make_hash_ref cs kp_bytes
+
+val key_package_ref_to_index: #l:nat -> #n:tree_size l -> ciphersuite -> treesync l n -> key_package_ref_nt -> result (option (leaf_index n))
+let key_package_ref_to_index #l #n cs t kp_ref =
+  let leaves = get_leaf_list t in
+  kp_refs <-- mapM (fun (_, olp) ->
+    match olp with
+    | Some lp -> (
+        kp_ref <-- leaf_package_to_kp_ref cs lp;
+        return (Some kp_ref)
+    )
+    | None -> return None
+  ) leaves;
+  let opt_res = (find_first (fun x -> x = Some kp_ref) kp_refs) in
+  return #(option (leaf_index n)) opt_res
